coq/Completeness.v
@@ -264,7 +264,30 @@ Proof.
     apply IHe with (ot := (Some t1)) in H4.
     destruct (eval_exp c_ls c_gs (Some t1) e) as [dv | ] eqn:E.
     {
+      (* TODO: avoid duplicate blocks *)
       inversion H1; subst.
+      {
+        inversion H4; subst.
+        destruct t1; try apply OA_None.
+        destruct t2;
+        try (
+          simpl;
+          repeat (destruct w; try apply OA_None);
+          destruct (make_dynamic_int sort (smt_eval_ast m sort ast)); apply OA_None
+        ).
+        {
+          rename w into w1, w0 into w2.
+          repeat (destruct w1; try apply OA_None);
+          (
+            simpl;
+            destruct sort; try apply OA_None;
+            repeat (destruct w2; try apply OA_None);
+            simpl;
+            eapply OA_Some;
+            [ reflexivity | reflexivity ]
+          ).
+        }
+      }
       {
         inversion H4; subst.
         destruct t1; try apply OA_None.
